open import Size 

open import Data.Nat 
open import Data.Nat.Properties
open import Data.Fin hiding (_â‰¤_; _+_)
open import Data.Vec hiding (map; [_]; _>>=_)
open import Data.Bool
open import Data.List hiding (fromMaybe)
open import Data.Maybe hiding (fromMaybe; map)
open import Data.Empty
open import Data.Product using (uncurry; _,_; âˆƒ; âˆƒ-syntax; _Ã—_; Î£; Î£-syntax)

import Relation.Binary.PropositionalEquality as Eq'
open Eq' using (_â‰¡_; refl; cong; sym; trans)
open Eq'.â‰¡-Reasoning using (begin_; _â‰¡âŸ¨âŸ©_; _â‰¡âŸ¨_âŸ©_; _âˆ)

open import AgdaGen.Base
open import AgdaGen.Combinators

open import Function

open import Category.Monad

module AgdaGen.Indexed.Examples where 
  
  fin : ğ”¾áµ¢ Fin
  fin zero    = None
  fin (suc n) = â¦‡ zero          â¦ˆ
              âˆ¥ â¦‡ suc (` fin n) â¦ˆ

  prop : âŸ¨ fin 5 âŸ© 10 â‰¡
    zero âˆ·
    suc zero âˆ·
    suc (suc zero) âˆ·
    suc (suc (suc zero)) âˆ· suc (suc (suc (suc zero))) âˆ· []
  prop = refl

  
  â‰¤m : ğ”¾áµ¢ (uncurry _â‰¤_)
  â‰¤m (zero  , m    ) = â¦‡ zâ‰¤n â¦ˆ
  â‰¤m (suc n , zero ) = None
  â‰¤m (suc n , suc m) = â¦‡ sâ‰¤s (` â‰¤m (n , m)) â¦ˆ
  
  â‰¤-suc : âˆ€ {n m : â„•} â†’ n â‰¤ m â†’ n â‰¤ suc m
  â‰¤-suc zâ‰¤n = zâ‰¤n
  â‰¤-suc (sâ‰¤s p) = sâ‰¤s (â‰¤-suc p)

  {-
  â‰¤n+k : ğ”¾áµ¢ (Î» p â†’ fst p â‰¤ snd p + fst p)
  â‰¤n+k (n , zero ) = â¦‡ (â‰¤-reflexive refl)      â¦ˆ
  â‰¤n+k (n , suc k) = â¦‡ â‰¤-suc (` â‰¤n+k (n , k))  â¦ˆ

  
  vec : âˆ€ {a : Set} â†’ âŸª ğ”¾ a âŸ« â†’ âŸª ğ”¾áµ¢ (Vec a) âŸ«
  vec a Î¼ zero    = â¦‡ []            â¦ˆ
  vec a Î¼ (suc n) = â¦‡ âŸ¨ a âŸ© âˆ· (Î¼ n) â¦ˆ

  data Sorted {â„“} : List â„• â†’ Set â„“ where
    nil    : Sorted []
    single : âˆ€ {n : â„•} â†’ Sorted (n âˆ· [])
    step   : âˆ€ {n m : â„•} {xs : List â„•} â†’ n â‰¤ m â†’ Sorted {â„“} (m âˆ· xs) â†’ Sorted {â„“} (n âˆ· m âˆ· xs)

  
  nâ‰¤m? : (n m : â„•) â†’ Maybe (n â‰¤ m)
  nâ‰¤m? zero m          = just zâ‰¤n
  nâ‰¤m? n zero          = nothing
  nâ‰¤m? (suc n) (suc m) = Data.Maybe.map sâ‰¤s (nâ‰¤m? n m)

  sortedâ‚› : âŸª ğ”¾áµ¢ Sorted âŸ«
  sortedâ‚› Î¼ []      = â¦‡ nil    â¦ˆ
  sortedâ‚› Î¼(x âˆ· []) = â¦‡ single â¦ˆ
  sortedâ‚› Î¼ (x âˆ· y âˆ· xs) with nâ‰¤m? x y
  sortedâ‚› Î¼ (x âˆ· y âˆ· xs) | nothing = uninhabited
  sortedâ‚› Î¼ (x âˆ· y âˆ· xs) | just p = â¦‡ (step p) (Î¼ (y âˆ· xs)) â¦ˆ

  bump : â„• â†’ List â„• â†’ List â„•
  bump n [] = []
  bump n (x âˆ· xs) = x + n âˆ· bump (x + n) xs

  Sorted' : âˆ€ {â„“} â†’ List â„• â†’ Set â„“
  Sorted' = Sorted âˆ˜ (bump 0) 

  nâ‰¤k+n : (n k : â„•) â†’ n â‰¤ k + n
  nâ‰¤k+n n zero = â‰¤-reflexive refl
  nâ‰¤k+n n (suc k) = â‰¤-suc (nâ‰¤k+n n k)

  nâ‰¤mâ†’n+kâ‰¤m+k : âˆ€ {n m k : â„•} â†’ n â‰¤ m â†’ n + k â‰¤ m + k
  nâ‰¤mâ†’n+kâ‰¤m+k {n = n} {m = m} {k = zero} p rewrite +-comm n 0 | +-comm m 0 = p
  nâ‰¤mâ†’n+kâ‰¤m+k {n = n} {m = m} {k = suc k} p rewrite +-suc n k | +-suc m k = sâ‰¤s (nâ‰¤mâ†’n+kâ‰¤m+k p)

  map-preserves-sorted : âˆ€ {â„“} {n : â„•} {xs : List â„•}
                         â†’ Sorted {â„“} xs
                         â†’ Sorted {â„“} (map (Î» x â†’ x + n) xs)
  map-preserves-sorted nil = nil
  map-preserves-sorted single = single
  map-preserves-sorted (step x prf) = step (nâ‰¤mâ†’n+kâ‰¤m+k x) (map-preserves-sorted prf)

  Sorted-eq : âˆ€ {â„“} {xs ys : List â„•} â†’ xs â‰¡ ys â†’ Sorted {â„“} xs â†’ Sorted {â„“} ys
  Sorted-eq refl sp = sp

  bump-map-eq : âˆ€ {n m : â„•} {xs : List â„•} â†’ map (Î» x â†’ x + m) (bump n xs) â‰¡ bump (n + m) xs
  bump-map-eq {xs = []} = refl
  bump-map-eq {n = n} {m = m} {xs = x âˆ· xs} rewrite sym (+-assoc x n m) =
    cong (_âˆ·_ (x + n + m)) (bump-map-eq {n = x + n} {m = m} {xs = xs})

  bump-lemma : âˆ€ {â„“} {n m : â„•} {xs : List â„•}
               â†’ Sorted {â„“} (bump n xs)
               â†’ Sorted {â„“} (bump (n + m) xs)
  bump-lemma {n = n} {m = m} {xs = xs} p  =
    Sorted-eq bump-map-eq (map-preserves-sorted {n = m} {xs = bump n xs} p)
  
  sorted : âŸª ğ”¾áµ¢ Sorted' âŸ«
  sorted Î¼ []           = â¦‡ nil â¦ˆ
  sorted Î¼ (x âˆ· [])     = â¦‡ single â¦ˆ
  sorted Î¼ (x âˆ· y âˆ· xs) rewrite +-comm x 0 =
    â¦‡ (step (nâ‰¤k+n x y) âˆ˜ bump-lemma {n = 0}) (Î¼ (y âˆ· xs)) â¦ˆ

  â‰¤-diff : âˆ€ {n m : â„•} â†’ n â‰¤ m â†’ â„•
  â‰¤-diff {zero} {m} p = m
  â‰¤-diff {suc n} {zero} ()
  â‰¤-diff {suc n} {suc m} (sâ‰¤s p) = suc (â‰¤-diff p)

  â‰¤-equivalence : âˆ€ {n m} â†’ n â‰¤ m
                  ----------------------------------------
                  â†’ âˆƒ[ k ] ((n â‰¤ (n + k)) âŠ— (m â‰¡ (n + k)))
                  
  â‰¤-equivalence {zero} {m} p = m , p , refl
  â‰¤-equivalence {suc n} {m = suc m} (sâ‰¤s p) with â‰¤-equivalence p
  â‰¤-equivalence {suc n} {suc .(n + k)} (sâ‰¤s p) | k , (leq , refl) =
    k , sâ‰¤s leq , refl

  bump-eq-lemma : âˆ€ {x y v : â„•} {xs ys : List â„•}
                  â†’ y âˆ· xs â‰¡ bump x (v âˆ· ys)
                  â†’ x âˆ· y âˆ· xs â‰¡ bump 0 (x âˆ· v âˆ· ys)
  bump-eq-lemma {x} refl rewrite +-comm x 0 = refl

  minus-0 : âˆ€ {n : â„•} â†’ âˆ£ n - 0 âˆ£ â‰¡ n
  minus-0 {zero} = refl
  minus-0 {suc n} = refl

  lemma-minus : âˆ€ {n m : â„•} â†’ n â‰¤ m â†’ âˆ£ m - n âˆ£ + n â‰¡ m
  lemma-minus {.0} {m} zâ‰¤n rewrite +-comm âˆ£ m - 0 âˆ£ 0 | minus-0 {n = m} = refl
  lemma-minus {(suc n)} {(suc m)} (sâ‰¤s p) with lemma-minus p
  ... | res rewrite +-suc âˆ£ m - n âˆ£ n = cong suc res

  lemma-sorted-â‰¤ : âˆ€ {â„“} {n m : â„•} {xs : List â„•} â†’ n â‰¤ m â†’ Sorted {â„“} (m âˆ· xs) â†’ Sorted {â„“} (n âˆ· xs)
  lemma-sorted-â‰¤ leq single = single
  lemma-sorted-â‰¤ {n = n} {m = m} leq (step x p) = step (â‰¤-trans leq x) p

  dfst : âˆ€ {â„“} {a : Set â„“} {P : a â†’ Set â„“} â†’ Î£ a P â†’ a
  dfst (x , _) = x
  
  {-
  sorted-equivalence : âˆ€ {â„“} {xs : List â„•} â†’ Sorted {â„“} xs
                       -----------------------------------------
                       â†’ âˆƒ[ ys ] (Sorted' ys âŠ— (xs â‰¡ bump 0 ys))
  sorted-equivalence {xs = []} nil = [] , nil , refl
  sorted-equivalence {xs = x âˆ· []} single rewrite +-comm 0 x = [ x ] , single , refl
  sorted-equivalence {xs = x âˆ· y âˆ· xs} (step leq p) = {!!}
  -}

  data Foo : â„• â†’ Set where
    bar : Foo zero
    baz : âˆ€ {n m : â„•} â†’ Foo n â†’ Foo m â†’ Foo (n + m)

  foo : âŸª ğ”¾áµ¢ Foo âŸ«
  foo Î¼ zero    = â¦‡ bar â¦ˆ âˆ¥ â¦‡ baz (Î¼ 0) (Î¼ 0) â¦ˆ
  foo Î¼ (suc n) = â¦‡ baz (Î¼ {!!}) (Î¼ {!!}) â¦ˆ

-}
